\documentclass[
  border=2,
  convert={
    density=100 -alpha remove,
    outext=.png
  },
]{standalone}
\usepackage{amsmath}
\begin{document}
\begin{tabular}{l}
  \begin{tabular}{l l l}
    $\displaystyle t_0 = D_0$ &
    $\displaystyle t_1 = D_0 + D_1$ &
    $\displaystyle t_2 = D_0 + D_1 + D_2$
  \end{tabular}
  \\ \\
  \begin{tabular}{l l}
    $\displaystyle f(x) = 2^{(n-1)} k \left(\frac{x}{D_1}\right)^{n}$ &
    $\displaystyle g(x) = k - f(D_1 - x)$
  \end{tabular}
  \\ \\
  $
    \displaystyle e(x) = \begin{cases}
      1
        & (0 \leq x \leq D_0) \\
      f(x - D_0) + 1
        & \left(D_0 \leq x \leq D_0 + \frac{D_1}{2}\right) \\
      g(x - D_0) + 1
        & \left(D_0 + \frac{D_1}{2} \leq x \leq D_1\right) \\
      K
        & (D_1 \leq x \leq D_2)
    \end{cases}
  $
  \\ \\
  \begin{tabular}{l l}
    $\displaystyle F(x) = \frac{2^{(n-1)}kx^{(n+1)}}{(n+1){D_1}^{n}}$ &
    $\displaystyle G(x) = k\left(x - \frac{D_1}{2}\right) + F(D_1-x)$
  \end{tabular}
  \\ \\
  $
    \displaystyle \int_0^x e(x) dx = \begin{cases}
      x              
        & (0  \leq x \leq D_0) \\
      F(x - D_0) + x
        & \left(D_0 \leq x \leq D_0 + \frac{D_1}{2}\right) \\
      G(x - D_0) + x
        & \left(D_0 + \frac{D_1}{2} \leq x \leq D_1\right) \\
      G(D_1) + k(x - (D_0 + D_1)) + x
        & (D_1 \leq x \leq D_2)
    \end{cases}
  $ 
\end{tabular}
\end{document}
